Fix lemma about `AArch64_TranslateAddress`
Also add assumption that monitor debug events are disabled in
`MDSCR_EL1` to simplify the handling of `AArch64_CheckDebug` (called in
address translation) and `SSAdvance` (called in the top-level step
function).

CHERI_Instantiation.thy
@@ -5999,7 +5999,8 @@ fun sysreg_ev_assms :: "(Capability, register_value) axiom_state \<Rightarrow> r
         (no_system_reg_access \<longrightarrow> \<not>cap_permits (CAP_PERM_EXECUTE OR CAP_PERM_SYSTEM) c))"
 | "sysreg_ev_assms s (E_read_reg r (Regval_bitvector_32_dec v)) =
      ((r = ''CSCR_EL3'' \<longrightarrow> no_system_reg_access \<or> v !! 0) \<and>
-      (r = ''EDSCR'' \<longrightarrow> (ucast v :: 6 word) = 2))" (* Non-debug state *)
+      (r = ''EDSCR'' \<longrightarrow> (ucast v :: 6 word) = 2) \<and> \<comment> \<open>Non-debug state\<close>
+      (r = ''MDSCR_EL1'' \<longrightarrow> (\<not>v !! 15))) \<comment> \<open>Monitor debug events disabled (breakpoints/watchpoints)\<close>"
 | "sysreg_ev_assms s (E_read_reg r (Regval_signal v)) =
      (r = ''DBGEN'' \<longrightarrow> v = LOW)" (* No external debugger *)
 | "sysreg_ev_assms s (E_read_reg r (Regval_ProcState v)) =
